***NO_CI*** making two phase tc a settable option, pointers now goes through, a single proof pattern was causing the 3 failures, but same pattern on small test cases goes through, need to debug more

src/basic/FStar.Options.fs
@@ -951,7 +951,8 @@ let settable = function
     | "reuse_hint_for"
     | "z3rlimit_factor"
     | "z3rlimit"
-    | "z3refresh" -> true
+    | "z3refresh"
+    | "use_two_phase_tc" -> true
     | _ -> false
 
 // the first two options below are options that are passed to z3 using
